src/linear/layer1/ADT.dfy
@@ -1,0 +1,23 @@
+trait ADT<M> {
+  function ReprDepth(): nat
+    ensures ReprDepth() > 0
+
+  function ReprFamily(n: nat): set<object>
+    decreases n
+    requires n <= ReprDepth()
+    ensures n > 0 ==> ReprFamily(n) >= ReprFamily(n-1)
+    reads this, if n == 0 then {} else ReprFamily(n-1)
+
+  function Repr(): set<object>
+    reads this, ReprFamily(ReprDepth()-1)
+  {
+    ReprFamily(ReprDepth())
+  }
+
+  predicate Valid()
+    reads this, Repr()
+
+  function Model(): M
+    reads this, Repr()
+    requires Valid()
+}
